theories/noetherian_wf.v
@@ -35,9 +35,9 @@ Section noetherian_wf.
 
   Implicit Type (l m k : list 𝓡).
 
-  Let T (P Q : 𝓡 → Prop) := Q ⊂w P ∧ ideal Q.
+  Let R (P Q : 𝓡 → Prop) := Q ⊂w P ∧ ideal Q.
 
-  Local Lemma bar_PA__Acc l : bar PA l → ¬ PA l → ∀P, ⌞l⌟ ⊆₁ P → Acc T P.
+  Local Lemma bar_PA__Acc l : bar PA l → ¬ PA l → ∀P, ⌞l⌟ ⊆₁ P → Acc R P.
   Proof.
     induction 1 as [ l Hl | l _ IHl ].
     + now intros [].
@@ -59,7 +59,7 @@ Section noetherian_wf.
       sequence of ideals of 𝓡 is terminating. *)
 
   Theorem noetherian__wf_strict_incl_rev :
-    well_founded T.
+    well_founded R.
   Proof.
     intro.
     apply bar_PA__Acc with (l := []); auto.
@@ -71,7 +71,7 @@ Section noetherian_wf.
     well_founded (λ P Q : sig (@ideal 𝓡), proj1_sig Q ⊂w proj1_sig P).
   Proof.
     generalize noetherian__wf_strict_incl_rev.
-    unfold T.
+    unfold R.
     wf rel morph (λ x y, x = proj1_sig y).
     + intros []; simpl; eauto.
     + intros ? ? [] []; simpl; intros; subst; auto.
@@ -86,7 +86,7 @@ Section noetherian_wf.
     + intros ? ? ? ? -> ->; auto.
   Qed.
 
-  Corollary noetherian__wf_fin_idl_strict_incl :
+  Corollary noetherian__wf_fg_idl_strict_incl :
     well_founded (λ l m : list 𝓡, idl ⌞m⌟ ⊂w idl ⌞l⌟).
   Proof.
     generalize noetherian__wf_idl_strict_incl.
@@ -94,10 +94,20 @@ Section noetherian_wf.
     + intros l; now exists ⌞l⌟.
     + intros ? ? ? ? -> ->; auto.
   Qed.
+  
+  Corollary noetherian__wf_strict_incl_fg_ideal :
+    well_founded (λ P Q : sig (@fg_ideal 𝓡), proj1_sig Q ⊂w proj1_sig P).
+  Proof.
+    generalize noetherian__wf_strict_incl_ideal.
+    wf rel morph (λ x y, proj1_sig x = proj1_sig y).
+    + intros (f & Hf); simpl; now exists (exist _ _ (fg_ideal__ideal Hf)).
+    + intros ? ? [] []; simpl; intros; subst; auto.
+  Qed.
 
 End noetherian_wf.
 
 Arguments noetherian__wf_strict_incl_rev {_}.
 Arguments noetherian__wf_strict_incl_ideal {_}.
 Arguments noetherian__wf_idl_strict_incl {_}.
-Arguments noetherian__wf_fin_idl_strict_incl {_}.
+Arguments noetherian__wf_fg_idl_strict_incl {_}.
+Arguments noetherian__wf_strict_incl_fg_ideal {_}.
